#+title: Worksheet 4
#+author: Ethan Coe-Renner

* Notes
- f(x_1,x_2,x_3) = \prod{}M(1,5,7)
- 001 101 111
- (x_1 + x_2 + x_3') (x_1' + x_2 + x_3') (x_1' + x_2' + x_3')
- (x_1 + x_2 + x_3') (x_1' + x_2 + x_3') (x_1' + x_2 + x_3') (x_1' + x_2' + x_3') 
- (x_2 + x_3') (x_1' + x_3')

* Problems
1. f(x_1 , x_2 , x_3) = \prod{}M(2,4,6)
   1. 
       | x_1 | x_2 | x_3 | f |
       |-----+-----+-----+---|
       |   0 |   0 |   0 | 1 |
       |   0 |   0 |   1 | 1 |
       |   0 |   1 |   0 | 0 |
       |   0 |   1 |   1 | 1 |
       |   1 |   0 |   0 | 0 |
       |   1 |   0 |   1 | 1 |
       |   1 |   1 |   0 | 0 |
       |   1 |   1 |   1 | 1 |
   2. (010 100 110)

      f(x_1 , x_2 , x_3) = (x_1 + x_2' + x_3) (x_1' + x_2 + x_3) (x_1' + x_2' x_3)
   3. 
      f(x_1 , x_2 , x_3) = (x_1 + x_2' + x_3) (x_1' + x_2 + x_3) (x_1' + x_2' x_3)

      f(x_1 , x_2 , x_3) = (x_1 + x_2' + x_3) (x_1' + x_2 + x_3) (x_1' + x_2' x_3) (x_1' + x_2' x_3)

      combine terms 1, 4 and 2,3
  
      f(x_1 , x_2 , x_3) = (x_2' + x_3) (x_1' + x_3)

   4. 
       [[./Ws4-1.jpeg]]

       cost = 2(2) + 2(2 + 2(2)) + 2 + 2(2) = 22

2. f(x_1 , x_2 , x_3) = \prod{}M(0,1,6,7)

   1. 
       | x_1 | x_2 | x_3 | f |
       |-----+-----+-----+---|
       |   0 |   0 |   0 | 0 |
       |   0 |   0 |   1 | 0 |
       |   0 |   1 |   0 | 1 |
       |   0 |   1 |   1 | 1 |
       |   1 |   0 |   0 | 1 |
       |   1 |   0 |   1 | 1 |
       |   1 |   1 |   0 | 0 |
       |   1 |   1 |   1 | 0 |

   2. SOP, the 1's in the truth table are closer together, so maybe they will be easier to combine

   3. f(x_1 , x_2 , x_3) = x_1' x_2 x_3' + x_1' x_2 x_3 + x_1 x_2' x_3' + x_1 x_2' x_3

   4. f(x_1 , x_2 , x_3) = x_1' x_2 x_3' + x_1' x_2 x_3 + x_1 x_2' x_3' + x_1 x_2' x_3

      combine terms 1, 2 and 3,4

      f(x_1 , x_2 , x_3) = x_1' x_2 + x_1 x_2'

   5.
      [[./Ws4-2.jpeg]]

      cost = 2(2) + 2(2 + 2(2)) + 2 +  2(2) = 22
